Prove correction (in a certain sense) of nested trees
An important part of the TreeBasedRefinement example is to swap from a
filter over the list of elements to a find over the tree structure. This
was previously justified by manual proofs relying on the KeyedOnPID
predicate; this commit subsumes these proofs by introducing a
bfind_correct predicate in the Bag interface, and proving this predicate
for both the fmap- and the list-based implementations.

The bag interface now has two extra fields, bfind_matcher and
bfind_correct; bfind_matcher is a boolean function which, used in
conjunction with a search toer to filter over the results of benumerate,
must return the same as calling bfind directly.

bstar is the empty search term (such that find bstar == benumerate (the
bstar_search predicate).

ADTExamples/QueryStructure/Bags/Bags.v
@@ -26,9 +26,14 @@ Proof.
   intros [ seq ( [ eq_head | in_seqs ] & in_seq ) ]; subst; eauto.
 Qed.
 
+Require Import SetEq.
+
 Class Bag (TContainer TItem TSearchTerm: Type) :=
   {
-    bempty     : TContainer;
+    bempty        : TContainer;
+    bstar         : TSearchTerm;
+    bfind_matcher : TSearchTerm -> TItem -> bool;
+
     benumerate : TContainer -> list TItem;
     bfind      : TContainer -> TSearchTerm -> list TItem;
     binsert    : TContainer -> TItem -> TContainer;
@@ -36,7 +41,12 @@ Class Bag (TContainer TItem TSearchTerm: Type) :=
     binsert_enumerate : forall item inserted container,
                           List.In item (benumerate (binsert container inserted)) <->
                           List.In item (benumerate container) \/ item = inserted;
-    benumerate_empty  : forall item, ~ List.In item (benumerate bempty)
+    benumerate_empty  : forall item, ~ List.In item (benumerate bempty);
+    bstar_search      : forall container, bfind container bstar = benumerate container;
+    bfind_correct     : forall container search_term,
+                          SetEq
+                            (List.filter (bfind_matcher search_term) (benumerate container))
+                            (bfind container search_term)
   }.
 
 Module IndexedTree (Import M: WS).
@@ -65,6 +75,12 @@ Module IndexedTree (Import M: WS).
       iconsistency : IndexedBagConsistency projection ifmap
     }.
 
+  Definition KeyFilter 
+             {TItem}
+             (key: TKey)
+             (projection: TItem -> TKey) :=
+    (fun x : TItem => if E.eq_dec (projection x) key then true else false).
+      
   Definition EmptyAsIndexedBag 
              (TBag TItem TBagSearchTerm: Type) 
              (bags_bag: Bag TBag TItem TBagSearchTerm) projection 
@@ -139,6 +155,16 @@ Module IndexedTree (Import M: WS).
         bempty := 
           EmptyAsIndexedBag TBag TItem TBagSearchTerm bags_bag projection;
 
+        bstar  :=
+          (None, @bstar _ _ _ bags_bag);
+
+        bfind_matcher key_searchterm item :=
+          let (key_option, search_term) := key_searchterm in
+          match key_option with
+            | Some k => KeyFilter k projection item
+            | None   => true 
+          end && (bfind_matcher search_term item);
+
         benumerate container :=
           flatten (List.map benumerate (Values (container.(ifmap))));
 
@@ -160,10 +186,8 @@ Module IndexedTree (Import M: WS).
           {|
             ifmap := add k (bag.(binsert) item) container.(ifmap);
             iconsistency := _
-          |};
-
-        binsert_enumerate := _
-      |}.
+          |}
+      |}. 
     Proof.
       intros; simpl in *.
 
@@ -174,7 +198,7 @@ Module IndexedTree (Import M: WS).
 
       split; intro H.
       
-      destruct H as [ items ( [ bag (bag_items & [ key maps_to ]) ] & in_seq ) ].
+      destruct H as [ items ( in_seq & [ bag (bag_items & [ key maps_to ]) ] ) ].
       pose proof maps_to as maps_to'.
       rewrite add_mapsto_iff in maps_to;
         destruct maps_to as [(is_eq & refreshed) | (neq & maps_to)].
@@ -206,13 +230,13 @@ Module IndexedTree (Import M: WS).
       Focus 2.
       unfold flatten, EmptyAsIndexedBag; simpl.
       rewrite Values_empty; tauto.
-
-      destruct H as [ [ items ( [ bag ( bag_items & [ key maps_to ] ) ] ) ] | eq_item_inserted ].
+ 
+      destruct H as [ [ items ( in_seq & [ bag ( bag_items & [ key maps_to ] ) ] ) ] | eq_item_inserted ].
       
       pose proof maps_to as maps_to'.
       apply (iconsistency container) in maps_to.    
       setoid_rewrite bag_items in maps_to.
-      specialize (maps_to item H).
+      specialize (maps_to item in_seq).
       
       setoid_rewrite add_mapsto_iff.
 
@@ -245,13 +269,407 @@ Module IndexedTree (Import M: WS).
       end.
 
       exists (benumerate v).
-      split.
-      exists v; split; trivial.
-      exists k.
 
-      apply add_1; trivial.
+      split.
+
       unfold v.
       rewrite binsert_enumerate; auto.
+
+      exists v; split; trivial.
+      exists k.
+      apply add_1; trivial.
+
+      intros; induction (Values (ifmap container)); simpl; trivial.
+      rewrite (@bstar_search _ _ _ bags_bag).
+      f_equal; trivial.
+
+
+      intros.
+      destruct search_term as (option_key, search_term).
+      destruct option_key as [ key | ].
+
+      (* Key provided *)
+
+      pose (iconsistency container).
+      unfold IndexedBagConsistency in i.
+
+
+      Lemma filter_and :
+        forall {A} pred1 pred2,
+        forall (seq: list A),
+          List.filter (fun x => pred1 x && pred2 x) seq =
+          List.filter pred1 (List.filter pred2 seq).
+      Proof.
+        intros; 
+        induction seq;
+        simpl;
+        [ | destruct (pred1 a) eqn:eq1; 
+            destruct (pred2 a) eqn:eq2];
+        simpl; 
+        try rewrite eq1;
+        try rewrite eq2;
+        trivial;
+        f_equal;
+        trivial.
+      Qed.
+
+      Lemma filter_and_opp :
+        forall {A} pred1 pred2,
+        forall (seq: list A),
+          List.filter (fun x => pred1 x && pred2 x) seq =
+          List.filter pred2 (List.filter pred1 seq).
+      Proof.
+        intros; 
+        induction seq;
+        simpl;
+        [ | destruct (pred1 a) eqn:eq1; 
+            destruct (pred2 a) eqn:eq2];
+        simpl; 
+        try rewrite eq1;
+        try rewrite eq2;
+        trivial;
+        f_equal;
+        trivial.
+      Qed.
+
+      rewrite filter_and_opp.
+
+      Lemma flatten_filter :
+        forall {A} (seq: list (list A)) pred, 
+          List.filter pred (flatten seq) =
+          flatten (List.map (List.filter pred) seq). 
+      Proof.
+        intros; induction seq; trivial.
+        unfold flatten; simpl.
+        induction a; trivial.
+        simpl; 
+          destruct (pred a); simpl; rewrite IHa; trivial.
+      Qed.
+
+      rewrite flatten_filter.
+      
+
+        Lemma equiv_eq_key_elt :
+          forall elt,
+            Equivalence (eq_key_elt (elt:=elt)).
+        Proof.
+          intros; unfold eq_key_elt; intuition.
+          unfold Symmetric; firstorder.
+          unfold Transitive; firstorder.
+          transitivity (fst y); trivial.
+          transitivity (snd y); trivial.
+        Qed.
+
+        Lemma equiv_eq_key :
+          forall elt,
+            Equivalence (eq_key (elt:=elt)).
+        Proof.
+          intros; unfold eq_key; intuition.
+          unfold Transitive; firstorder.
+          transitivity (fst y); trivial.
+        Qed.
+
+
+        Lemma map_map :
+          forall { A B C } (proc1: A -> B) (proc2: B -> C),
+            forall seq,
+            List.map proc2 (List.map proc1 seq) = List.map (fun x => proc2 (proc1 x)) seq.
+        Proof.            
+          intros; induction seq; simpl; f_equal; trivial.
+        Qed.        
+   
+        Lemma InA_front_InA :
+          forall elt,
+          forall {item} front middle tail,
+            InA (eq_key_elt (elt:=elt)) item front -> InA (eq_key_elt (elt:=elt)) item (front ++ middle :: tail).
+        Proof.
+          intros; intuition. 
+          rewrite InA_app_iff;
+            [intuition | apply equiv_eq_key_elt].
+        Qed.
+
+        Lemma InA_tail_InA :
+          forall elt,
+          forall {item} front middle tail,
+            InA (eq_key_elt (elt:=elt)) item tail -> InA (eq_key_elt (elt:=elt)) item (front ++ middle :: tail).
+        Proof.
+          intros; intuition. 
+          rewrite InA_app_iff;
+            [intuition | apply equiv_eq_key_elt].
+        Qed.
+
+        Lemma InA_front_tail_InA :
+          forall elt,
+          forall {item} front middle tail,
+            InA (eq_key_elt (elt:=elt)) item front \/ InA (eq_key_elt (elt:=elt)) item tail -> 
+            InA (eq_key_elt (elt:=elt)) item (front ++ middle :: tail).
+        Proof.
+          intros elt item front middle tail in_or;
+          destruct in_or; eauto using InA_front_InA, InA_tail_InA.
+        Qed.
+        
+      Lemma consist :
+        forall 
+          {TBag TItem TSearchTerm bags_bag projection} 
+          (container: @IndexedBag TBag TItem TSearchTerm bags_bag projection),
+        forall k,
+          eq
+            (flatten
+               (List.map (List.filter (KeyFilter k projection))
+                         (List.map benumerate (Values (ifmap container)))))
+            match find k (ifmap container) with
+              | Some bag => benumerate bag
+              | None => []
+            end.
+      Proof.          
+        intros.
+        
+        pose (iconsistency container); unfold IndexedBagConsistency in i.
+        unfold Values.
+        destruct (find k (ifmap container)) as [ bag | ] eqn:eqfind.
+
+        rewrite <- find_mapsto_iff in eqfind.
+        (* assert (exists k', MapsTo k' bag (ifmap container)) as eqfind' by (exists k; trivial).*)
+
+        pose proof eqfind as maps_to.
+
+        rewrite elements_mapsto_iff in eqfind.
+        apply InA_split in eqfind.
+
+        destruct eqfind as [ l1 [ y [ l2 (y_k_bag & decomp) ] ] ].
+        rewrite decomp.
+        
+        rewrite (map_map snd benumerate).
+        rewrite ! map_app; simpl.
+        
+        pose proof (elements_3w (ifmap container)) as no_dup.
+        rewrite decomp in no_dup; apply NoDupA_swap in no_dup; eauto using equiv_eq_key.
+        Print NoDupA.
+        inversion no_dup as [ | ? ? y_not_in no_dup' ]; subst.
+        rewrite InA_app_iff in y_not_in by eauto using equiv_eq_key.
+     
+        unfold eq_key_elt in y_k_bag; simpl in y_k_bag.
+        destruct y_k_bag as (y_k & y_bag).
+
+        assert (forall k' bag', InA (@eq_key_elt _) (k', bag') (l1 ++ l2) -> 
+                                   forall item, 
+                                     List.In item (benumerate bag') ->
+                                     ~ E.eq (projection item) k).
+        {
+          intros k' bag' in_app item in_bag'_items eq_k.
+
+          rewrite InA_app_iff in in_app; eauto using equiv_eq_key_elt.
+          pose proof in_app as in_app'.
+
+          apply (InA_front_tail_InA _ _ y) in in_app.
+          rewrite <- decomp, <- elements_mapsto_iff in in_app.
+
+          pose proof (i _ _ in_app _ in_bag'_items) as eq_k'. 
+          symmetry in eq_k.
+          pose proof (E.eq_trans eq_k eq_k').
+
+          assert (eq_key y (k', bag')) as y_eq by (unfold eq_key; simpl; eauto).
+
+          destruct in_app' as [ in_seq | in_seq ];
+            (apply (InA_eqke_eqk (k2 := fst y) (snd y)) in in_seq; eauto);
+            rewrite <- surjective_pairing in in_seq; intuition.
+        }
+
+        Lemma filter_all_true :
+          forall {A} pred (seq: list A),
+            (forall x, List.In x seq -> pred x = true) ->
+            List.filter pred seq = seq.
+        Proof.
+          induction seq as [ | head tail IH ]; simpl; trivial.
+          intros all_true.
+          rewrite all_true by eauto.
+          f_equal; intuition.
+        Qed.
+
+        Lemma filter_all_false :
+          forall {A} seq pred,
+            (forall item : A, List.In item seq -> pred item = false) ->
+            List.filter pred seq = [].
+        Proof.
+          intros A seq pred all_false; induction seq as [ | head tail IH ]; simpl; trivial.
+          rewrite (all_false head) by (simpl; eauto). 
+          intuition.
+        Qed.
+
+        Lemma map_filter_all_false :
+          forall {A} pred seq, 
+            (forall subseq, List.In subseq seq -> 
+                            forall (item: A), List.In item subseq -> 
+                                              pred item = false) ->
+            (List.map (List.filter pred) seq) = (List.map (fun x => []) seq).
+        Proof.
+          intros A pred seq all_false; 
+          induction seq as [ | subseq subseqs IH ] ; simpl; trivial.
+          
+          f_equal.
+
+          specialize (all_false subseq (or_introl eq_refl)).
+          apply filter_all_false; assumption.
+
+          apply IH; firstorder.
+        Qed.
+
+        Lemma flatten_nils :
+          forall {A} (seq: list (list A)),
+            flatten (List.map (fun _ => []) seq) = @nil A.
+        Proof.        
+          induction seq; intuition. 
+        Qed.
+
+        Lemma flatten_app :
+          forall {A} (seq1 seq2: list (list A)),
+            flatten (seq1 ++ seq2) = flatten seq1 ++ flatten seq2.
+        Proof.
+          unfold flatten; induction seq1; simpl; trivial.
+          intros; rewrite IHseq1; rewrite app_assoc; trivial.
+        Qed.
+
+        Lemma flatten_head :
+          forall {A} head tail,
+            @flatten A (head :: tail) = head ++ flatten tail.
+        Proof.
+          intuition.
+        Qed.
+        
+        Ltac destruct_if :=
+          match goal with
+              [ |- context [ if ?cond then _ else _ ] ] => destruct cond
+          end.
+
+        Lemma KeyFilter_true :
+          forall {A} k projection (item: A),
+            KeyFilter k projection item = true <-> E.eq (projection item) k.
+        Proof.
+          unfold KeyFilter; intros;
+          destruct_if; intros; intuition.
+        Qed.
+
+        Lemma KeyFilter_false :
+          forall {A} k projection (item: A),
+            KeyFilter k projection item = false <-> ~ E.eq (projection item) k.
+        Proof.
+          unfold KeyFilter; intros;
+          destruct_if; intros; intuition.
+        Qed.
+
+        Lemma In_InA :
+          forall (A : Type) (l : list A) (eqA : relation A) (x : A),
+            Equivalence eqA -> List.In x l -> InA eqA x l.
+        Proof.
+          induction l; intros; simpl in *.
+          exfalso; eauto using in_nil.
+          destruct H0.
+          apply InA_cons_hd; subst; reflexivity.
+          apply InA_cons_tl, IHl; trivial.
+        Qed.
+
+        rewrite ! map_filter_all_false;
+          [ | intros subseq in_map item in_subseq;
+              rewrite in_map_iff in in_map;
+              destruct in_map as [ (k', bag') (benum_eq & in_seq) ];
+              rewrite KeyFilter_false;
+              
+              simpl in benum_eq;
+              subst subseq;
+              apply (H k' bag'); 
+              eauto;
+              
+              apply In_InA; eauto using equiv_eq_key_elt;
+              rewrite in_app_iff;
+              eauto 
+                .. ].
+
+        rewrite 
+          flatten_app, 
+          flatten_head, 
+          !flatten_nils, 
+          app_nil_l, app_nil_r, 
+          <- y_bag,
+          filter_all_true; trivial.
+
+        intros;
+        rewrite KeyFilter_true;
+        apply (iconsistency container _ bag); eauto.
+
+        Lemma nil_in_false :
+          forall {A} seq,
+            seq = [] <-> ~ exists (x: A), List.In x seq.
+        Proof.
+          split; intro H.
+          intros [ x in_seq ]; subst; eauto using in_nil.
+          destruct seq as [ | a ]; trivial.
+          exfalso; apply H; exists a; simpl; intuition.
+        Qed.
+        
+        rewrite nil_in_false.
+        intros [item item_in].
+
+        rewrite in_flatten_iff in item_in.
+        do 2 setoid_rewrite in_map_iff in item_in.
+
+        destruct item_in as 
+            [ subseq 
+                (in_subseq 
+                   & [ subseq_prefilter 
+                         ( pre_post_filter 
+                             & [ bag 
+                                   (eq_bag_pre_filter 
+                                      & bag_in) ] ) ] ) ].
+
+        subst subseq.
+        rewrite filter_In in in_subseq.
+        destruct in_subseq as (in_subseq_prefilter & key_filter).
+
+        rewrite KeyFilter_true in key_filter.
+        rewrite <- MapsTo_snd in bag_in.
+        destruct bag_in as [k' maps_to].
+
+        subst.
+        rewrite <- key_filter in eqfind.
+        rewrite <- (iconsistency container k' bag maps_to _ in_subseq_prefilter) in maps_to.
+        rewrite find_mapsto_iff in maps_to.
+
+        congruence.
+      Qed.
+
+      Show.
+      rewrite consist.
+      destruct (find key (ifmap container)) as [ bag | ].
+
+      apply bfind_correct.
+      eauto using SetEq_Reflexive.
+
+      (* No key provided *)
+
+      rewrite flatten_filter.
+
+      induction (Values (ifmap container)); simpl.
+
+      compute; tauto.
+
+      rewrite IHl.
+
+      Lemma SetEq_app :
+        forall {A: Type} (s1 t1 s2 t2: list A),
+          (SetEq s1 s2) /\ (SetEq t1 t2) -> SetEq (s1 ++ t1) (s2 ++ t2).
+      Proof.
+        unfold SetEq; 
+        intros A s1 t1 s2 t2 (s1s2 & t1t2); 
+        split;
+        rewrite ! in_app_iff;
+        intro inApp;
+        [ rewrite s1s2, t1t2 in inApp
+        | rewrite <- s1s2, <- t1t2 in inApp ];
+        trivial.
+      Qed.
+
+      apply SetEq_app; split; eauto using SetEq_Reflexive.
+      apply bfind_correct.
 
       Grab Existential Variables.
       intros k' bag' maps_to item'.
@@ -280,23 +698,28 @@ Module IndexedTree (Import M: WS).
 
       apply (iconsistency container k' bag' maps_to item').
     Defined.
-
-    Print Assumptions IndexedBagAsBag. 
 End IndexedTree.
 
 Instance ListAsBag
          {TItem TSearchTerm: Type}
+         (star: TSearchTerm)
          (matcher: TSearchTerm -> TItem -> bool)
+         (star_search: forall (i: TItem), matcher star i = true)
 : Bag (list TItem) TItem TSearchTerm.
 Proof.
   refine (
       {| 
-        bempty := []; 
+        bempty := [];
+        bstar  := star;
         benumerate := id;
         bfind container search_term := List.filter (matcher search_term) container;
         binsert container item := cons item container
       |}
     ); simpl in *; intuition.
+
+  unfold id.
+  induction container; simpl; trivial.
+  rewrite star_search, IHcontainer; trivial.
 Defined.
 
 Require Import Tuple Heading.
@@ -331,7 +754,7 @@ Definition TupleEqualityMatcher
 Instance TupleListAsBag (heading: Heading) :
   Bag (list (@Tuple heading)) (@Tuple heading) (SearchTermsCollection heading).
 Proof.
-  apply (ListAsBag (@MatchAgainstSearchTerms heading)).
+  apply (ListAsBag [] (@MatchAgainstSearchTerms heading)); eauto.
 Defined.
 
 Require Import Beatles.
@@ -342,11 +765,11 @@ Require Import String_as_OT.
 Open Scope string_scope.
 Open Scope Tuple_scope.
 
+(*
 Eval simpl in (bfind FirstAlbums [ TupleEqualityMatcher (eq_dec := string_dec) Name "Please Please Me" ]).
-
 Eval simpl in (bfind FirstAlbums [ TupleEqualityMatcher (eq_dec := eq_nat_dec) Year 3]).
-
 Eval simpl in (bfind FirstAlbums [ TupleEqualityMatcher (eq_dec := eq_nat_dec) Year 3; TupleEqualityMatcher (eq_dec := eq_nat_dec) UKpeak 1]).
+*)
 
 Module NatIndexedMap := FMapAVL.Make Nat_as_OT.
 Module StringIndexedMap := FMapAVL.Make String_as_OT.
@@ -391,14 +814,14 @@ Fixpoint NestedTreeFromAttributes'
       {| BagType        := list (@Tuple heading);
          SearchTermType := SearchTermsCollection heading |}
     | proper_attr :: more_indexes => 
-      let attr := Attribute proper_attr in
+      let attr := @Attribute heading proper_attr in
       let (t, st, bagproof) := NestedTreeFromAttributes' heading more_indexes in
-      match (ProperlyTyped proper_attr) with
-        | left eq_nat     => 
-          {| BagType        := NatTreeType t st heading bagproof (fun x => cast eq_nat x!attr);
-             SearchTermType := option nat * st |}
+      match (@ProperlyTyped heading proper_attr) with
+        | left  eq_nat    => 
+          {| BagType        := NatTreeType    t st heading bagproof (fun x => cast eq_nat    (x attr));
+             SearchTermType := option nat    * st |}
         | right eq_string => 
-          {| BagType        := StringTreeType t st heading bagproof (fun x => cast eq_string x!attr);
+          {| BagType        := StringTreeType t st heading bagproof (fun x => cast eq_string (x attr));
              SearchTermType := option string * st |}
       end
     end.
@@ -445,7 +868,7 @@ Ltac mkIndex heading attributes :=
   set (source := attributes);
   assert (list (@ProperAttribute heading)) as decorated_source;
   autoconvert (@CheckType heading);
-  apply (NestedTreeFromAttributes' AlbumHeading decorated_source).
+  apply (NestedTreeFromAttributes' heading decorated_source).
 
 Definition SampleIndex : BagPlusBagProof AlbumHeading.
 Proof.
@@ -468,6 +891,7 @@ Time Eval simpl in (bfind IndexedAlbums (None, (None, (Some "With the Beatles", 
 Time Eval simpl in (bfind IndexedAlbums (None, (None, (None, [TupleEqualityMatcher (eq_dec := string_dec) Name "With the Beatles"])))).
 
 (*Time Eval simpl in (@bfind _ _ _ (BagProof _ SampleIndex) IndexedAlbums (Some 3, (Some 1, (None, @nil (TSearchTermMatcher AlbumHeading))))).*)
+*)
 
 (*
   simpl.
